@prefix : <https://w3id.org/ontouml#> .
@prefix dct: <http://purl.org/dc/terms/> .
@prefix owl: <http://www.w3.org/2002/07/owl#> .
@prefix rdf: <http://www.w3.org/1999/02/22-rdf-syntax-ns#> .
@prefix xml: <http://www.w3.org/XML/1998/namespace> .
@prefix xsd: <http://www.w3.org/2001/XMLSchema#> .
@prefix dcat: <http://www.w3.org/ns/dcat#> .
@prefix rdfs: <http://www.w3.org/2000/01/rdf-schema#> .
@prefix vann: <http://purl.org/vocab/vann/> .
@prefix ontouml: <https://w3id.org/ontouml#> .
@base <https://w3id.org/ontouml> .

<https://w3id.org/ontouml> rdf:type owl:Ontology ;
                            owl:versionIRI <https://w3id.org/ontouml/1.0> ;
                            dct:contributor <https://orcid.org/0000-0003-2736-7817> ,
                                            <https://orcid.org/0000-0003-3385-4769> ;
                            dct:creator <https://orcid.org/0000-0002-5385-5761> ,
                                        <https://orcid.org/0000-0003-2528-3118> ;
                            dct:description "A reference implementation of the OntoUML Metamodel in OWL."@en ;
                            dct:identifier "https://w3id.org/ontouml"^^xsd:anyURI ;
                            dct:isReferencedBy <https://dblp.org/rec/conf/jowo/FonsecaSVFGA21.html> ,
                                               <https://doi.org/10.1007/978-3-031-17995-2_1> ;
                            dct:issued "2022-04-03"^^xsd:date ;
                            dct:license <https://creativecommons.org/licenses/by-sa/4.0> ;
                            dct:modified "2023-04-27"^^xsd:date ;
                            dct:title "OntoUML Metamodel Vocabulary"@en ;
                            dct:conformsTo: <https://purl.org/krdb-core/ontouml-js> ;
                            dct:language: "en" ;
                            vann:preferredNamespacePrefix "ontouml"@en ;
                            vann:preferredNamespaceUri "https://w3id.org/ontouml#"^^xsd:anyURI ;
                            owl:versionInfo "1.1"@en ;
                            dcat:keyword "Metamodel"@en ,
                                         "OntoUML"@en ,
                                         "OntoUML-Metamodel"@en ,
                                         "OntoUML-Schema"@en ,
                                         "OntoUML-Vocabulary"@en ,
                                         "Ontology-Driven Conceptual Modeling"@en ;
                            dcat:landingPage <https://w3id.org/ontouml/git> .

#################################################################
#    Annotation properties
#################################################################

###  http://purl.org/dc/terms/conformsTo
dct:conformsTo rdf:type owl:AnnotationProperty .


###  http://purl.org/dc/terms/contributor
dct:contributor rdf:type owl:AnnotationProperty .


###  http://purl.org/dc/terms/creator
dct:creator rdf:type owl:AnnotationProperty .


###  http://purl.org/dc/terms/description
dct:description rdf:type owl:AnnotationProperty .


###  http://purl.org/dc/terms/identifier
dct:identifier rdf:type owl:AnnotationProperty .


###  http://purl.org/dc/terms/isReferencedBy
dct:isReferencedBy rdf:type owl:AnnotationProperty .


###  http://purl.org/dc/terms/issued
dct:issued rdf:type owl:AnnotationProperty .


###  http://purl.org/dc/terms/language
dct:language rdf:type owl:AnnotationProperty .


###  http://purl.org/dc/terms/license
dct:license rdf:type owl:AnnotationProperty .


###  http://purl.org/dc/terms/modified
dct:modified rdf:type owl:AnnotationProperty .


###  http://purl.org/dc/terms/title
dct:title rdf:type owl:AnnotationProperty .


###  http://purl.org/dc/terms/conformsTo:
dct:conformsTo: rdf:type owl:AnnotationProperty .


###  http://purl.org/dc/terms/language:
dct:language: rdf:type owl:AnnotationProperty .


###  http://purl.org/vocab/vann/preferredNamespacePrefix
vann:preferredNamespacePrefix rdf:type owl:AnnotationProperty .


###  http://purl.org/vocab/vann/preferredNamespaceUri
vann:preferredNamespaceUri rdf:type owl:AnnotationProperty .


###  http://www.w3.org/ns/dcat#keyword
dcat:keyword rdf:type owl:AnnotationProperty .


###  http://www.w3.org/ns/dcat#landingPage
dcat:landingPage rdf:type owl:AnnotationProperty .


#################################################################
#    Datatypes
#################################################################

###  http://www.w3.org/1999/02/22-rdf-syntax-ns#langString
rdf:langString rdf:type rdfs:Datatype .


#################################################################
#    Object Properties
#################################################################

###  https://w3id.org/ontouml#aggregationKind
ontouml:aggregationKind rdf:type owl:ObjectProperty ;
                        rdfs:domain ontouml:Property ;
                        rdfs:range ontouml:AggregationKind ;
                        rdfs:comment "Characterizes an ontouml:Property with an ontouml:AggregationKind instance, i.e., indicates whether the ontouml:Property is a simple (ontouml:none), a shared (ontouml:shared), or a composite (ontouml:composite) property."@en .


###  https://w3id.org/ontouml#attribute
ontouml:attribute rdf:type owl:ObjectProperty ;
                  rdfs:subPropertyOf ontouml:property ;
                  rdfs:domain ontouml:Class ;
                  rdfs:range ontouml:Property ;
                  rdfs:comment "Indicates the instances of type ontouml:Property that are attributes of an ontouml:Class."@en .


###  https://w3id.org/ontouml#cardinality
ontouml:cardinality rdf:type owl:ObjectProperty ;
                    rdfs:domain ontouml:Property ;
                    rdfs:range ontouml:Cardinality ;
                    rdfs:comment "Identifies the individual that represents the cardinalities of an ontouml:Property."@en .


###  https://w3id.org/ontouml#categorizer
ontouml:categorizer rdf:type owl:ObjectProperty ;
                    rdfs:domain ontouml:GeneralizationSet ;
                    rdfs:range ontouml:Class ;
                    rdfs:comment "Is the type of the highest order. It classifies the specific types of generalization sets' generalizations."@en .


###  https://w3id.org/ontouml#containsModelElement
ontouml:containsModelElement rdf:type owl:ObjectProperty ;
                             rdfs:subPropertyOf ontouml:contents ;
                             rdfs:domain ontouml:Package ;
                             rdfs:range ontouml:ModelElement .


###  https://w3id.org/ontouml#containsView
ontouml:containsView rdf:type owl:ObjectProperty ;
                     rdfs:subPropertyOf ontouml:contents ;
                     rdfs:domain ontouml:Diagram ;
                     rdfs:range ontouml:ElementView .


###  https://w3id.org/ontouml#contents
ontouml:contents rdf:type owl:ObjectProperty ;
                 rdfs:domain ontouml:Diagram ;
                 rdfs:range ontouml:ElementView .


###  https://w3id.org/ontouml#diagram
ontouml:diagram rdf:type owl:ObjectProperty ;
                rdfs:domain ontouml:Project ;
                rdfs:range ontouml:Diagram ;
                rdfs:comment "Identifies which entities of type ontouml:Diagram are part of a given ontouml:Project."@en ,
                             "It is mapped to the OntoUML Metamodel's 'diagrams' relation betwen a Project and a Diagram."@en .


###  https://w3id.org/ontouml#general
ontouml:general rdf:type owl:ObjectProperty ;
                rdfs:domain ontouml:Generalization ;
                rdfs:range ontouml:Classifier ;
                rdfs:comment "Points to the target node of a generalization relation, namely it is used to link a generalization relation to the corresponding parent class."@en .


###  https://w3id.org/ontouml#generalization
ontouml:generalization rdf:type owl:ObjectProperty ;
                       rdfs:domain ontouml:GeneralizationSet ;
                       rdfs:range ontouml:Generalization ;
                       rdfs:comment "The relation used to associate a subclass with its parent class, usually to be associated with a generalization set."@en .


###  https://w3id.org/ontouml#isViewOf
ontouml:isViewOf rdf:type owl:ObjectProperty ;
                 rdfs:domain ontouml:ElementView ;
                 rdfs:range ontouml:ModelElement ;
                 rdfs:comment "Relates an ontouml:ElementView to the ontouml:ModelElement, indicating the representation of the latter's diagramation."@en .


###  https://w3id.org/ontouml#literal
ontouml:literal rdf:type owl:ObjectProperty ;
                rdfs:domain ontouml:Class ;
                rdfs:range ontouml:Literal ;
                rdfs:comment "Identifies an ontouml:Literal within an ontouml:Class that has ontouml:stereotype with ontouml:enumeration."@en .


###  https://w3id.org/ontouml#model
ontouml:model rdf:type owl:ObjectProperty ;
              rdfs:domain ontouml:Project ;
              rdfs:range ontouml:Package ;
              rdfs:comment "Identifies an ontouml:Package that is part of an ontouml:Project."@en .


###  https://w3id.org/ontouml#owner
ontouml:owner rdf:type owl:ObjectProperty ;
              rdfs:domain ontouml:Diagram ;
              rdfs:range ontouml:ModelElement ;
              rdfs:comment "Relates an ontouml:Diagram with the ontouml:ModelElement that it is part of."@en .


###  https://w3id.org/ontouml#point
ontouml:point rdf:type owl:ObjectProperty ;
              rdfs:domain ontouml:Path ;
              rdfs:range ontouml:Point ;
              rdfs:comment "The property used to build geometric objects out of points, a fundamental two-dimensional building block."@en .


###  https://w3id.org/ontouml#project
ontouml:project rdf:type owl:ObjectProperty ;
                rdfs:domain [ owl:intersectionOf ( [ rdf:type owl:Class ;
                                                     owl:unionOf ( ontouml:Diagram
                                                                   ontouml:DiagramElement
                                                                   ontouml:ModelElement
                                                                 )
                                                   ]
                                                   [ rdf:type owl:Class ;
                                                     owl:complementOf ontouml:Project
                                                   ]
                                                 ) ;
                              rdf:type owl:Class
                            ] ;
                rdfs:range ontouml:Project ;
                rdfs:comment "Relates every ontouml:OntoumlElement different than ontouml:Project to the ontouml:Project that it is part of."@en .


###  https://w3id.org/ontouml#property
ontouml:property rdf:type owl:ObjectProperty ;
                 rdfs:domain ontouml:Classifier ;
                 rdfs:range ontouml:Property ;
                 rdfs:comment "Identifies a property exhibited by instances of the classifier. If the classifier is a class, the property is an attribute. If the classifier is a relation, the property is a relation end."@en .


###  https://w3id.org/ontouml#propertyType
ontouml:propertyType rdf:type owl:ObjectProperty ;
                     rdfs:domain ontouml:Property ;
                     rdfs:range ontouml:Classifier ;
                     rdfs:comment "Identifies the individual of type ontouml:Class or ontouml:Relation (i.e., an ontouml:Classifier) to which the ontouml:Property refers to."@en ;
                     rdfs:seeAlso "https://sparxsystems.com/enterprise_architect_user_guide/15.2/automation/propertytype.html"^^xsd:anyURI .


###  https://w3id.org/ontouml#redefinesProperty
ontouml:redefinesProperty rdf:type owl:ObjectProperty ;
                          rdfs:domain ontouml:Property ;
                          rdfs:range ontouml:Property ;
                          rdfs:comment "Redefining property will replace any reference to a redefined property in the context of an instance of the specializing classifier. A property could be redefined to have a different name, visibility, type, and default value."@en .


###  https://w3id.org/ontouml#relationEnd
ontouml:relationEnd rdf:type owl:ObjectProperty ;
                    rdfs:subPropertyOf ontouml:property ;
                    rdfs:domain ontouml:Relation ;
                    rdfs:range ontouml:Property ;
                    rdfs:comment "Determines the target of a given relation."@en .


###  https://w3id.org/ontouml#restrictedTo
ontouml:restrictedTo rdf:type owl:ObjectProperty ;
                     rdfs:domain ontouml:Class ;
                     rdfs:range ontouml:OntologicalNature ;
                     rdfs:comment "Associates an ontouml:Class to an ontouml:OntologicalNature, restricting the allowed values for that ontouml:Class."@en .


###  https://w3id.org/ontouml#shape
ontouml:shape rdf:type owl:ObjectProperty ;
              rdfs:domain ontouml:ElementView ;
              rdfs:range ontouml:Shape ;
              rdfs:comment "Relates an ontouml:ElementView to the ontouml:Shape that contains the diagramation's data (size and position) about the ontouml:ModelElement it is a view of."@en .


###  https://w3id.org/ontouml#sourceEnd
ontouml:sourceEnd rdf:type owl:ObjectProperty ;
                  rdfs:subPropertyOf ontouml:relationEnd ;
                  rdfs:domain ontouml:Relation ;
                  rdfs:range ontouml:Property ;
                  rdfs:comment "Identifies the source class associated with a given relation."@en .


###  https://w3id.org/ontouml#sourceView
ontouml:sourceView rdf:type owl:ObjectProperty ;
                   rdfs:domain ontouml:ConnectorView ;
                   rdfs:range ontouml:ElementView ;
                   rdfs:comment "Is a shape in the source end of a relationView or generalizationView."@en .


###  https://w3id.org/ontouml#specific
ontouml:specific rdf:type owl:ObjectProperty ;
                 rdfs:domain ontouml:Generalization ;
                 rdfs:range ontouml:Classifier ;
                 rdfs:comment "Points to the source node of a generalization relation, namely it is used to link a generalization relation to the corresponding subclass."@en .


###  https://w3id.org/ontouml#stereotype
ontouml:stereotype rdf:type owl:ObjectProperty ;
                   rdfs:domain ontouml:DecoratableElement ;
                   rdfs:range ontouml:Stereotype ;
                   rdfs:comment "Identifies the stereotype applied to the decoratable."@en .


###  https://w3id.org/ontouml#subsetsProperty
ontouml:subsetsProperty rdf:type owl:ObjectProperty ;
                        rdfs:domain ontouml:Property ;
                        rdfs:range ontouml:Property ;
                        rdfs:comment "Links a property to its parent property."@en .


###  https://w3id.org/ontouml#targetEnd
ontouml:targetEnd rdf:type owl:ObjectProperty ;
                  rdfs:subPropertyOf ontouml:relationEnd ;
                  rdfs:domain ontouml:Relation ;
                  rdfs:range ontouml:Property ;
                  rdfs:comment "Identifies the target class associated with a given relation."@en .


###  https://w3id.org/ontouml#targetView
ontouml:targetView rdf:type owl:ObjectProperty ;
                   rdfs:domain ontouml:ConnectorView ;
                   rdfs:range ontouml:ElementView ;
                   rdfs:comment "Is a shape in the target end of a relationView or generalizationView."@en .


###  https://w3id.org/ontouml#text
ontouml:targetView rdf:type owl:ObjectProperty ;
                   rdfs:domain ontouml:Text ;
                   rdfs:range xsd:string ;
                   rdfs:comment "Relates a text message to its ontouml:Text container."@en .

###  https://w3id.org/ontouml#topLeftPosition
ontouml:topLeftPosition rdf:type owl:ObjectProperty ;
                        rdfs:domain ontouml:RectangularShape ;
                        rdfs:range ontouml:Point ;
                        rdfs:comment "Is direct mapped to the metamodel's 'topLeft' relationship between a RectangularShape and a Point."@en ,
                                     "Relates an ontouml:RectangularShape with an ontouml:Point that contains the horizontal (x) and vertical (y) coordinates representing the former's top left position."@en .


#################################################################
#    Data properties
#################################################################

###  https://w3id.org/ontouml#cardinalityValue
ontouml:cardinalityValue rdf:type owl:DatatypeProperty ;
                         rdfs:domain ontouml:Cardinality ;
                         rdfs:range xsd:string ;
                         rdfs:comment "Provides the complete (i.e., both lower and upper cardinality's bounds) cardinalities of a given ontouml:Property via its related ontouml:Cardinality."@en .


###  https://w3id.org/ontouml#description
ontouml:description rdf:type owl:DatatypeProperty ;
                    rdfs:domain ontouml:OntoumlElement ;
                    rdfs:range [ rdf:type rdfs:Datatype ;
                                 owl:unionOf ( rdf:langString
                                               xsd:string
                                             )
                               ] ;
                    rdfs:comment "A non-empty nullable string representing the description of the object in free textual format."@en .


###  https://w3id.org/ontouml#height
ontouml:height rdf:type owl:DatatypeProperty ;
               rdfs:domain ontouml:RectangularShape ;
               rdfs:range xsd:positiveInteger ;
               rdfs:comment "Indicates the height of an ontouml:RectangularShape that is represented in an ontouml:Diagram."@en .


###  https://w3id.org/ontouml#isAbstract
ontouml:isAbstract rdf:type owl:DatatypeProperty ;
                   rdfs:domain ontouml:Classifier ;
                   rdfs:range xsd:boolean ;
                   rdfs:comment "Identifies if the classifier can have direct instances. If set to true, the classifier must be specialized before being instantiated. Otherwise, it can have direct instances."@en .


###  https://w3id.org/ontouml#isComplete
ontouml:isComplete rdf:type owl:DatatypeProperty ;
                   rdfs:domain ontouml:GeneralizationSet ;
                   rdfs:range xsd:boolean ;
                   rdfs:comment "Describes if a generalization set is complete, namely it does not admit further generalizations."@en .


###  https://w3id.org/ontouml#isDerived
ontouml:isDerived rdf:type owl:DatatypeProperty ;
                  rdfs:domain ontouml:DecoratableElement ;
                  rdfs:range xsd:boolean ;
                  rdfs:comment "Identifies if the extension of the classifier or the value of a property can be \"computed\" through a derivation rule. For instance, the class Child can be modeled as a derived class if defined as a person whose age is less or equal to 10."@en .


###  https://w3id.org/ontouml#isDisjoint
ontouml:isDisjoint rdf:type owl:DatatypeProperty ;
                   rdfs:domain ontouml:GeneralizationSet ;
                   rdfs:range xsd:boolean ;
                   rdfs:comment "Describes if a generalization set is disjoint, namely it does not admit generalizations having overlapping subclasses."@en .


###  https://w3id.org/ontouml#isExtensional
ontouml:isExtensional rdf:type owl:DatatypeProperty ;
                      rdfs:domain ontouml:Class ;
                      rdfs:range xsd:boolean ;
                      rdfs:comment "Identifies if an ontouml:CollectiveClass is extensionally defined (i.e., it's parts cannot change)."@en .


###  https://w3id.org/ontouml#isOrdered
ontouml:isOrdered rdf:type owl:DatatypeProperty ;
                  rdfs:domain ontouml:Property ;
                  rdfs:range xsd:boolean ;
                  rdfs:comment "Indicates if a collection is ordered or not. If the attribute represents a database column, this represents a primary key when set."@en .


###  https://w3id.org/ontouml#isPowertype
ontouml:isPowertype rdf:type owl:DatatypeProperty ;
                    rdfs:domain ontouml:Class ;
                    rdfs:range xsd:boolean ;
                    rdfs:comment "Identifies if an ontouml:Class is a powertype in multi-level modeling."@en ,
                                 "The ontouml:Class data property ontouml:isPowertype must not be true when it has an ontouml:order equal to one."@en .


###  https://w3id.org/ontouml#isReadOnly
ontouml:isReadOnly rdf:type owl:DatatypeProperty ;
                   rdfs:domain ontouml:Property ;
                   rdfs:range xsd:boolean ;
                   rdfs:comment "Denotes when a property may or may not be updated or modified."@en .


###  https://w3id.org/ontouml#lowerBound
ontouml:lowerBound rdf:type owl:DatatypeProperty ;
                   rdfs:domain ontouml:Cardinality ;
                   rdfs:range xsd:nonNegativeInteger ;
                   rdfs:comment "Identifies the lower bound of a ontouml:Cardinality."@en,
                   "A ontouml:Cardinality's lower bound must correspond to the one indicated by its ontouml:cardinalityValue property." ,
                   "E.g., if the cardinality set is [1..*] then the lower bound is '1'."@en .


###  https://w3id.org/ontouml#name
ontouml:name rdf:type owl:DatatypeProperty ;
             rdfs:domain ontouml:OntoumlElement ;
             rdfs:range [ rdf:type rdfs:Datatype ;
                          owl:unionOf ( rdf:langString
                                        xsd:string
                                      )
                        ] ;
             rdfs:comment "A non-empty nullable string containing the object's name. It is allowed for two objects of the ontology to have identical names, even if they are of the same type."@en .


###  https://w3id.org/ontouml#order
ontouml:order rdf:type owl:DatatypeProperty ;
              rdfs:domain ontouml:Class ;
              rdfs:range xsd:nonNegativeInteger ;
              rdfs:comment "Constraint: an ontouml:Class decorated with an ontouml:stereotype different than ontouml:type must have an ontouml:order value equal to 1."@en ,
                           "Constraint: an ontouml:Class decorated with the ontouml:stereotype ontouml:type must have an ontouml:order value grater than 1."@en ,
                           "Identifies the order of a class enabling multi-level modeling."@en .


###  https://w3id.org/ontouml#upperBound
ontouml:upperBound rdf:type owl:DatatypeProperty ;
                   rdfs:domain ontouml:Cardinality ;
                   rdfs:range rdfs:Literal ;
                   rdfs:comment "Identifies the upper bound of a ontouml:Cardinality."@en,
                   "A ontouml:Cardinality's upper bound must correspond to the one indicated by its ontouml:cardinalityValue property." ,
                   "E.g., if the cardinality set is [1..*] then the upper bound is '*'."@en .


###  https://w3id.org/ontouml#width
ontouml:width rdf:type owl:DatatypeProperty ;
              rdfs:domain ontouml:RectangularShape ;
              rdfs:range xsd:positiveInteger ;
              rdfs:comment "Indicates the width of an ontouml:RectangularShape that is represented in an ontouml:Diagram."@en .


###  https://w3id.org/ontouml#xCoordinate
ontouml:xCoordinate rdf:type owl:DatatypeProperty ;
          rdfs:domain ontouml:Point ;
          rdfs:range xsd:integer ;
          rdfs:comment "Is direct mapped to the metamodel's 'x' attribute of the Point class."@en ,
                       "Relates an ontouml:Point to the value indicating the specific x (horizontal) coordinate of the top left position of an ontouml:RectangularShape."@en .


###  https://w3id.org/ontouml#yCoordinate
ontouml:yCoordinate rdf:type owl:DatatypeProperty ;
          rdfs:domain ontouml:Point ;
          rdfs:range xsd:integer ;
          rdfs:comment "Is direct mapped to the metamodel's 'y' attribute of the Point class."@en ,
                       "Relates an ontouml:Point to the value indicating the specific y (vertical) coordinate of the top left position of an ontouml:RectangularShape."@en .


#################################################################
#    Classes
#################################################################

###  https://w3id.org/ontouml#AggregationKind
ontouml:AggregationKind rdf:type owl:Class ;
                        owl:equivalentClass [ rdf:type owl:Class ;
                                              owl:oneOf ( ontouml:composite
                                                          ontouml:none
                                                          ontouml:shared
                                                        )
                                            ] ;
                        rdfs:comment "The class grouping the aggregation kinds of a given property."@en .


###  https://w3id.org/ontouml#Cardinality
ontouml:Cardinality rdf:type owl:Class ;
              rdfs:comment "Represents the cardinality of an ontouml:Property throught its data property ontouml:cardinalityValue."@en .



###  https://w3id.org/ontouml#Class
ontouml:Class rdf:type owl:Class ;
              rdfs:subClassOf ontouml:Class ,
                              ontouml:Classifier ;
              rdfs:comment "An object representing a type defined in the ontology."@en .

###  https://w3id.org/ontouml#CollectiveClass
ontouml:Class rdf:type owl:Class ;
              rdfs:subClassOf ontouml:Class ,
                              ontouml:Classifier ;
              rdfs:comment "Is an ontouml:Class that has the ontouml:stereotype property value ontouml:collective."@en .


###  https://w3id.org/ontouml#ClassStereotype
ontouml:ClassStereotype rdf:type owl:Class ;
                        owl:equivalentClass [ rdf:type owl:Class ;
                                              owl:oneOf ( ontouml:abstract
                                                          ontouml:category
                                                          ontouml:collective
                                                          ontouml:datatype
                                                          ontouml:enumeration
                                                          ontouml:event
                                                          ontouml:historicalRole
                                                          ontouml:historicalRoleMixin
                                                          ontouml:kind
                                                          ontouml:mixin
                                                          ontouml:mode
                                                          ontouml:phase
                                                          ontouml:phaseMixin
                                                          ontouml:quality
                                                          ontouml:quantity
                                                          ontouml:relator
                                                          ontouml:role
                                                          ontouml:roleMixin
                                                          ontouml:situation
                                                          ontouml:subkind
                                                          ontouml:type
                                                        )
                                            ] ;
                        rdfs:subClassOf ontouml:Stereotype ;
                        rdfs:comment "Aggregates all possible instances that can be assigned vian ontouml:stereotype object property to an ontouml:Class."@en .


###  https://w3id.org/ontouml#ClassView
ontouml:ClassView rdf:type owl:Class ;
                  rdfs:subClassOf ontouml:NodeView ;
                  rdfs:comment "Does not directly contain data about the visual representation (rectangular shape size and position) itself, but is related to this information via the ontouml:shape property."@en ,
                               "Represents the diagramation (i.e., the visual representation) of an ontouml:Class in a given ontouml:Diagram."@en .


###  https://w3id.org/ontouml#Classifier
ontouml:Classifier rdf:type owl:Class ;
                   rdfs:subClassOf ontouml:DecoratableElement ;
                   owl:disjointUnionOf ( ontouml:Class
                                         ontouml:Relation
                                       ) .


###  https://w3id.org/ontouml#ConnectorView
ontouml:ConnectorView rdf:type owl:Class ;
                      rdfs:subClassOf ontouml:ElementView ;
                      owl:disjointUnionOf ( ontouml:GeneralizationView
                                            ontouml:RelationView
                                          ) ;
                      rdfs:comment "The view of a given connector in a given diagram of a given model."@en .


###  https://w3id.org/ontouml#DecoratableElement
ontouml:DecoratableElement rdf:type owl:Class ;
                           rdfs:subClassOf ontouml:ModelElement ;
                           owl:disjointUnionOf ( ontouml:Classifier
                                                 ontouml:Property
                                               ) .


###  https://w3id.org/ontouml#Diagram
ontouml:Diagram rdf:type owl:Class ;
                rdfs:subClassOf ontouml:OntoumlElement ;
                rdfs:comment "Identifies a visual representation of an OntoUML model or of a portion of it."@en .


###  https://w3id.org/ontouml#DiagramElement
ontouml:DiagramElement rdf:type owl:Class ;
                       rdfs:subClassOf ontouml:OntoumlElement ;
                       owl:disjointUnionOf ( ontouml:ElementView
                                             ontouml:Shape
                                           ) ;
                       rdfs:comment "Identifies a diagram model element."@en .


###  https://w3id.org/ontouml#ElementView
ontouml:ElementView rdf:type owl:Class ;
                    rdfs:subClassOf ontouml:DiagramElement ;
                    owl:disjointUnionOf ( ontouml:ConnectorView
                                          ontouml:GeneralizationSetView
                                          ontouml:NodeView
                                        ) ;
                    rdfs:comment "E.g., an ontouml:ClassView is created whenever an ontouml:ModelElement is represented in an ontouml:Diagram."@en ,
                                 "Represents the diagramatical representation of an element in an ontouml:Diagram."@en .


###  https://w3id.org/ontouml#Generalization
ontouml:Generalization rdf:type owl:Class ;
                       rdfs:subClassOf ontouml:ModelElement ;
                       rdfs:comment "An object representing a generalization defined in the ontology."@en .


###  https://w3id.org/ontouml#GeneralizationSet
ontouml:GeneralizationSet rdf:type owl:Class ;
                          rdfs:subClassOf ontouml:ModelElement ;
                          rdfs:comment "An object representing a generalization set defined in the ontology."@en .


###  https://w3id.org/ontouml#GeneralizationSetView
ontouml:GeneralizationSetView rdf:type owl:Class ;
                              rdfs:subClassOf ontouml:ElementView ;
                              rdfs:comment "The view of a generalizationSet in a given diagram of a given model."@en .


###  https://w3id.org/ontouml#GeneralizationView
ontouml:GeneralizationView rdf:type owl:Class ;
                           rdfs:subClassOf ontouml:ConnectorView ;
                           rdfs:comment "The view of a generalization in a given diagram of a given model."@en .


###  https://w3id.org/ontouml#Literal
ontouml:Literal rdf:type owl:Class ;
                rdfs:subClassOf ontouml:ModelElement ;
                rdfs:comment "An object representing a value defined for an enumeration."@en .


###  https://w3id.org/ontouml#ModelElement
ontouml:ModelElement rdf:type owl:Class ;
                     rdfs:subClassOf ontouml:OntoumlElement ;
                     owl:disjointUnionOf ( ontouml:DecoratableElement
                                           ontouml:Generalization
                                           ontouml:GeneralizationSet
                                           ontouml:Literal
                                           ontouml:Package
                                         ) ;
                     rdfs:comment "Identifies a model element."@en .


###  https://w3id.org/ontouml#NodeView
ontouml:NodeView rdf:type owl:Class ;
                 rdfs:subClassOf ontouml:ElementView ;
                 owl:disjointUnionOf ( ontouml:ClassView
                                       ontouml:PackageView
                                     ) ;
                 rdfs:comment "The view of a node in a given diagram of a given model."@en .


###  https://w3id.org/ontouml#OntologicalNature
ontouml:OntologicalNature rdf:type owl:Class ;
                          owl:equivalentClass [ rdf:type owl:Class ;
                                                owl:oneOf ( ontouml:abstractNature
                                                            ontouml:collectiveNature
                                                            ontouml:eventNature
                                                            ontouml:extrinsicModeNature
                                                            ontouml:functionalComplexNature
                                                            ontouml:intrinsicModeNature
                                                            ontouml:qualityNature
                                                            ontouml:quantityNature
                                                            ontouml:relatorNature
                                                            ontouml:situationNature
                                                            ontouml:typeNature
                                                          )
                                              ] ;
                          rdfs:comment "Indicates the ontological nature of the individuals that the restricted type includes among its instances."@en .


###  https://w3id.org/ontouml#OntoumlElement
ontouml:OntoumlElement rdf:type owl:Class ;
                       owl:disjointUnionOf ( ontouml:Diagram
                                             ontouml:DiagramElement
                                             ontouml:ModelElement
                                             ontouml:Project
                                           ) .


###  https://w3id.org/ontouml#Package
ontouml:Package rdf:type owl:Class ;
                rdfs:subClassOf ontouml:ModelElement ;
                rdfs:comment "Aggregates ontology components or components of an ontology module, working as a container."@en .


###  https://w3id.org/ontouml#PackageView
ontouml:PackageView rdf:type owl:Class ;
                    rdfs:subClassOf ontouml:NodeView ;
                    rdfs:comment "A particular type of node view."@en .


###  https://w3id.org/ontouml#Path
ontouml:Path rdf:type owl:Class ;
             rdfs:subClassOf ontouml:Shape ;
             rdfs:comment "A list of connected points."@en .


###  https://w3id.org/ontouml#Point
ontouml:Point rdf:type owl:Class ;
              rdfs:comment "Datatype that contains the ontouml:xCoordinate value and ontouml:yCoordinate value. These values represent the top left position of an ontouml:RectangularShape, to which the ontouml:Point is related vian ontouml:topLeftPosition property."@en .


###  https://w3id.org/ontouml#Project
ontouml:Project rdf:type owl:Class ;
                rdfs:subClassOf ontouml:OntoumlElement ;
                rdfs:comment "Aggregates all entities that are part of a same conceptual model, including concepts declaration and their visual representation."@en ,
                             "It is the upper non-abstract class available in the OntoUML Vocabulary."@en .


###  https://w3id.org/ontouml#Property
ontouml:Property rdf:type owl:Class ;
                 rdfs:subClassOf ontouml:DecoratableElement ;
                 rdfs:comment "An object representing a property defined in the ontology. Properties contained by classes are deemed attributes and those contained by relations are deemed association ends."@en .


###  https://w3id.org/ontouml#PropertyStereotype
ontouml:PropertyStereotype rdf:type owl:Class ;
                           owl:equivalentClass [ rdf:type owl:Class ;
                                                 owl:oneOf ( ontouml:begin
                                                             ontouml:end
                                                           )
                                               ] ;
                           rdfs:subClassOf ontouml:Stereotype ;
                           rdfs:comment "A stereotype assigned to a property."@en .


###  https://w3id.org/ontouml#Rectangle
ontouml:Rectangle rdf:type owl:Class ;
                  rdfs:subClassOf ontouml:RectangularShape ;
                  rdfs:comment "A particular type of ontouml:RectangularShape, mainly used to represent entities of type ontouml:Class."@en .


###  https://w3id.org/ontouml#RectangularShape
ontouml:RectangularShape rdf:type owl:Class ;
                         rdfs:subClassOf ontouml:Shape ;
                         owl:disjointUnionOf ( ontouml:Rectangle
                                               ontouml:Text
                                             ) ;
                         rdfs:comment "Represents a rectangular shape in a given ontouml:Diagram."@en .


###  https://w3id.org/ontouml#Relation
ontouml:Relation rdf:type owl:Class ;
                 rdfs:subClassOf ontouml:Classifier ;
                 rdfs:comment "An object representing a relation defined in the ontology."@en .


###  https://w3id.org/ontouml#RelationStereotype
ontouml:RelationStereotype rdf:type owl:Class ;
                           owl:equivalentClass [ rdf:type owl:Class ;
                                                 owl:oneOf ( ontouml:bringsAbout
                                                             ontouml:characterization
                                                             ontouml:comparative
                                                             ontouml:componentOf
                                                             ontouml:creation
                                                             ontouml:derivation
                                                             ontouml:externalDependence
                                                             ontouml:historicalDependence
                                                             ontouml:instantiation
                                                             ontouml:manifestation
                                                             ontouml:material
                                                             ontouml:mediation
                                                             ontouml:memberOf
                                                             ontouml:participation
                                                             ontouml:participational
                                                             ontouml:subCollectionOf
                                                             ontouml:subQuantityOf
                                                             ontouml:termination
                                                             ontouml:triggers
                                                           )
                                               ] ;
                           rdfs:subClassOf ontouml:Stereotype ;
                           rdfs:comment "A stereotype assigned to a relation."@en .


###  https://w3id.org/ontouml#RelationView
ontouml:RelationView rdf:type owl:Class ;
                     rdfs:subClassOf ontouml:ConnectorView .


###  https://w3id.org/ontouml#Shape
ontouml:Shape rdf:type owl:Class ;
              rdfs:subClassOf ontouml:DiagramElement ;
              owl:disjointUnionOf ( ontouml:Path
                                    ontouml:RectangularShape
                                  ) ;
              rdfs:comment "The ontouml:DiagramElement that contains information about the diagramation of an ontouml:ModelElement through its relation with an ontouml:ModelView."@en .


###  https://w3id.org/ontouml#Stereotype
ontouml:Stereotype rdf:type owl:Class ;
                   owl:disjointUnionOf ( ontouml:ClassStereotype
                                         ontouml:PropertyStereotype
                                         ontouml:RelationStereotype
                                       ) ;
                   rdfs:comment "Indicates meta-properties of classes, properties, or relations."@en .


###  https://w3id.org/ontouml#Text
ontouml:Text rdf:type owl:Class ;
             rdfs:subClassOf ontouml:RectangularShape ;
             rdfs:comment "A rectangular shape used to introduce some text."@en ;
             rdfs:comment "TODO: STILL TO BE TREATED."@en .


###  https://w3id.org/ontouml#contents
ontouml:contents rdf:type owl:Class ;
                 owl:equivalentClass [ rdf:type owl:Class ;
                                       owl:unionOf ( ontouml:containsModelElement
                                                     ontouml:containsView
                                                   )
                                     ] .


#################################################################
#    Individuals
#################################################################

###  https://w3id.org/ontouml#abstract
ontouml:abstract rdf:type owl:NamedIndividual ,
                          ontouml:ClassStereotype ;
                 rdfs:comment "Represents the value of the ClassStereotype enumeration used to assign the corresponding stereotype Abstract to a given Class."@en .


###  https://w3id.org/ontouml#abstractNature
ontouml:abstractNature rdf:type owl:NamedIndividual ,
                                ontouml:OntologicalNature ;
                       rdfs:comment "Indicates that the restricted type includes abstract individuals among its instances."@en .


###  https://w3id.org/ontouml#begin
ontouml:begin rdf:type owl:NamedIndividual ,
                       ontouml:PropertyStereotype ;
              rdfs:comment "Identifies a stereotype that models the creation of an endurant."@en .


###  https://w3id.org/ontouml#bringsAbout
ontouml:bringsAbout rdf:type owl:NamedIndividual ,
                             ontouml:RelationStereotype .


###  https://w3id.org/ontouml#category
ontouml:category rdf:type owl:NamedIndividual ,
                          ontouml:ClassStereotype ;
                 rdfs:comment "A rigid mixin that does not require a dependency to be specified. It is used to aggregate essential properties of individuals following different identity principles."@en ;
                 rdfs:seeAlso "https://ontouml.readthedocs.io/en/latest/classes/nonsortals/category/index.html"^^xsd:anyURI .


###  https://w3id.org/ontouml#characterization
ontouml:characterization rdf:type owl:NamedIndividual ,
                                  ontouml:RelationStereotype ;
                         rdfs:comment "A relation between a bearer type and its feature. A feature is an intrinsic (inherent) moment of its bearer type, and thus existentially dependent on the bearer. A feature may be stereotyped as Quality or Mode. Feature characterizes a bearer type if and only if every instance of bearer exemplifies the feature."@en ;
                         rdfs:seeAlso "https://ontouml.readthedocs.io/en/latest/relationships/characterization/index.html"^^xsd:anyURI .


###  https://w3id.org/ontouml#collective
ontouml:collective rdf:type owl:NamedIndividual ,
                            ontouml:ClassStereotype ;
                   rdfs:comment "A construct used to represent rigid concepts that provide an identity principle for their instances. The main characteristic of a Collective is that it has a homogenous internal structure, i.e., all parts are perceived in the same way by the whole (see the MemberOf relation for more details about members of collections)."@en ;
                   rdfs:seeAlso "https://ontouml.readthedocs.io/en/latest/classes/sortals/collective/index.html"^^xsd:anyURI .


###  https://w3id.org/ontouml#collectiveNature
ontouml:collectiveNature rdf:type owl:NamedIndividual ,
                                  ontouml:OntologicalNature ;
                         rdfs:comment "Indicates that the restricted type includes collective individuals among its instances."@en .


###  https://w3id.org/ontouml#comparative
ontouml:comparative rdf:type owl:NamedIndividual ,
                             ontouml:RelationStereotype ;
                    rdfs:comment "The stereotype for comparative relations (e.g., heavier-than). Decorates functional relations that always hold between any two individuals bearing the same relevant quality."@en .


###  https://w3id.org/ontouml#componentOf
ontouml:componentOf rdf:type owl:NamedIndividual ,
                             ontouml:RelationStereotype ;
                    rdfs:comment "A parthood relation between two complexes."@en ;
                    rdfs:seeAlso "https://ontouml.readthedocs.io/en/latest/relationships/aggregations/componentOf/index.html"^^xsd:anyURI .


###  https://w3id.org/ontouml#composite
ontouml:composite rdf:type owl:NamedIndividual ,
                           ontouml:AggregationKind ;
                  rdfs:comment "The value denoting that an ontouml:Property represents a composite aggregation, namely a strong form of aggregation."@en .


###  https://w3id.org/ontouml#creation
ontouml:creation rdf:type owl:NamedIndividual ,
                          ontouml:RelationStereotype .


###  https://w3id.org/ontouml#datatype
ontouml:datatype rdf:type owl:NamedIndividual ,
                          ontouml:ClassStereotype ;
                 rdfs:comment "A classification that specifies which type of value a variable has and what type of mathematical, relational, or logical operations can be applied to it without causing an error."@en .


###  https://w3id.org/ontouml#derivation
ontouml:derivation rdf:type owl:NamedIndividual ,
                            ontouml:RelationStereotype .


###  https://w3id.org/ontouml#end
ontouml:end rdf:type owl:NamedIndividual ,
                     ontouml:PropertyStereotype ;
            rdfs:comment "Identifies a stereotype that models the termination of an endurant."@en .


###  https://w3id.org/ontouml#enumeration
ontouml:enumeration rdf:type owl:NamedIndividual ,
                             ontouml:ClassStereotype ;
                    rdfs:comment "A class represented with the enumeration stereotype having values represented using the field literals."@en .


###  https://w3id.org/ontouml#event
ontouml:event rdf:type owl:NamedIndividual ,
                       ontouml:ClassStereotype ;
              rdfs:comment "Things that happen to or are performed by endurants (Casati and Varzi, 2015)."@en ;
              rdfs:seeAlso "https://plato.stanford.edu/archives/win2015/entries/events/"^^xsd:anyURI .


###  https://w3id.org/ontouml#eventNature
ontouml:eventNature rdf:type owl:NamedIndividual ,
                             ontouml:OntologicalNature ;
                    rdfs:comment "Indicates that the restricted type includes event individuals among its instances."@en .


###  https://w3id.org/ontouml#externalDependence
ontouml:externalDependence rdf:type owl:NamedIndividual ,
                                    ontouml:RelationStereotype ;
                           rdfs:comment "Identifies an endurant on which the extrinsicMode depends."@en ;
                           rdfs:seeAlso "https://nemo-ufes.github.io/gufo/#externallyDependsOn"^^xsd:anyURI .


###  https://w3id.org/ontouml#extrinsicModeNature
ontouml:extrinsicModeNature rdf:type owl:NamedIndividual ,
                                     ontouml:OntologicalNature ;
                            rdfs:comment "Identifies what inheres in a concrete individual and depends on others for its existence."@en .


###  https://w3id.org/ontouml#functionalComplexNature
ontouml:functionalComplexNature rdf:type owl:NamedIndividual ,
                                         ontouml:OntologicalNature ;
                                rdfs:comment "Identifies the nature of a complex object whose parts (components) play different roles in its composition."@en .


###  https://w3id.org/ontouml#historicalDependence
ontouml:historicalDependence rdf:type owl:NamedIndividual ,
                                      ontouml:RelationStereotype ;
                             rdfs:comment "Identifies a concrete individual on which another concrete individual depends historically."@en .


###  https://w3id.org/ontouml#historicalRole
ontouml:historicalRole rdf:type owl:NamedIndividual ,
                                ontouml:ClassStereotype ;
                       rdfs:comment "Denotes the role of an endurant in virtue of having participated in an event of a particular type."@en .


###  https://w3id.org/ontouml#historicalRoleMixin
ontouml:historicalRoleMixin rdf:type owl:NamedIndividual ,
                                     ontouml:ClassStereotype ;
                            rdfs:comment "Denotes the equivalent of historicalRole for types that aggregate instances with different identity principles."@en .


###  https://w3id.org/ontouml#instantiation
ontouml:instantiation rdf:type owl:NamedIndividual ,
                               ontouml:RelationStereotype .


###  https://w3id.org/ontouml#intrinsicModeNature
ontouml:intrinsicModeNature rdf:type owl:NamedIndividual ,
                                     ontouml:OntologicalNature ;
                            rdfs:comment "Indicates that the restricted type includes intrinsic mode individuals among its instances."@en .


###  https://w3id.org/ontouml#kind
ontouml:kind rdf:type owl:NamedIndividual ,
                      ontouml:ClassStereotype ;
             rdfs:comment "A construct to be used in most of your models. It is used to represent rigid concepts that provide an identity principle for their instances and do not require a relational dependency. A Kind represents a Functional Complex, i.e., a whole that has parts contributing in different ways to its functionality (see the ComponentOf relation for more details about functional parts)."@en ;
             rdfs:seeAlso "https://ontouml.readthedocs.io/en/latest/classes/sortals/kind/index.html"^^xsd:anyURI .


###  https://w3id.org/ontouml#manifestation
ontouml:manifestation rdf:type owl:NamedIndividual ,
                               ontouml:RelationStereotype .


###  https://w3id.org/ontouml#material
ontouml:material rdf:type owl:NamedIndividual ,
                          ontouml:RelationStereotype ;
                 rdfs:comment "Identifies relations that have material structure on their own and include examples such as employments, kisses, enrollments, flight, connections and commitments. The relata of a material relation are mediated by individuals that are called relators."@en ;
                 rdfs:seeAlso "https://ontouml.readthedocs.io/en/latest/relationships/material/index.html"^^xsd:anyURI .


###  https://w3id.org/ontouml#mediation
ontouml:mediation rdf:type owl:NamedIndividual ,
                           ontouml:RelationStereotype ;
                  rdfs:comment "A type of existential dependence relation (a form of nonfunctional inherence). It can be derived from the relation between the relata and the qua individuals that compose the relator and that inhere in the relata."@en ;
                  rdfs:seeAlso "https://ontouml.readthedocs.io/en/latest/relationships/mediation/index.html"^^xsd:anyURI .


###  https://w3id.org/ontouml#memberOf
ontouml:memberOf rdf:type owl:NamedIndividual ,
                          ontouml:RelationStereotype ;
                 rdfs:comment "A parthood relation between a functional complex or a Collective (as a part) and a Collective (as a whole)."@en ;
                 rdfs:seeAlso "https://ontouml.readthedocs.io/en/latest/relationships/aggregations/memberOf/index.html"^^xsd:anyURI .


###  https://w3id.org/ontouml#mixin
ontouml:mixin rdf:type owl:NamedIndividual ,
                       ontouml:ClassStereotype ;
              rdfs:comment "A Mixin is a semi-rigid type, i.e., it behaves as a rigid type for some individuals and as an anti-rigid one for others (its the only stereotype with such a feature in OntoUML)."@en ;
              rdfs:seeAlso "https://ontouml.readthedocs.io/en/latest/classes/nonsortals/mixin/index.html"^^xsd:anyURI .


###  https://w3id.org/ontouml#mode
ontouml:mode rdf:type owl:NamedIndividual ,
                      ontouml:ClassStereotype ;
             rdfs:comment "A particular type of intrinsic property that has no structured value."@en ;
             rdfs:seeAlso "https://ontouml.readthedocs.io/en/latest/classes/aspects/mode/index.html"^^xsd:anyURI .


###  https://w3id.org/ontouml#none
ontouml:none rdf:type owl:NamedIndividual ,
                      ontouml:AggregationKind ;
             rdfs:comment "Denotes that a ontouml:Property is neither ontouml:shared nor ontouml:composite, but just an aggregation."@en .


###  https://w3id.org/ontouml#participation
ontouml:participation rdf:type owl:NamedIndividual ,
                               ontouml:RelationStereotype ;
                      rdfs:comment "A relation for representing when an event depends on a single object."@en .


###  https://w3id.org/ontouml#participational
ontouml:participational rdf:type owl:NamedIndividual ,
                                 ontouml:RelationStereotype ;
                        rdfs:comment "Denotes a kind of event decomposition."@en .


###  https://w3id.org/ontouml#phase
ontouml:phase rdf:type owl:NamedIndividual ,
                       ontouml:ClassStereotype ;
              rdfs:comment "A stereotype used to represent anti-rigid subtypes of identity providers (Kind, Collective, Quantity, Relator, Mode, and Quantity) that are instantiated by changes in intrinsic properties (e.g., the age of a person, the color of an object, the condition of a car). All instances of a particular Phase must follow the same identity principle. Phases always come in partitions."@en ;
              rdfs:seeAlso "https://ontouml.readthedocs.io/en/latest/classes/sortals/phase/index.html"^^xsd:anyURI .


###  https://w3id.org/ontouml#phaseMixin
ontouml:phaseMixin rdf:type owl:NamedIndividual ,
                            ontouml:ClassStereotype ;
                   rdfs:comment "The equivalent of Phase for types that aggregate instances with different identity principles. A class stereotyped as PhaseMixin is also an anti-rigid type. PhaseMixin is similar semantically to RoleMixin with the difference in relational dependency."@en ;
                   rdfs:seeAlso "https://ontouml.readthedocs.io/en/latest/classes/nonsortals/phasemixin/index.html"^^xsd:anyURI .


###  https://w3id.org/ontouml#quality
ontouml:quality rdf:type owl:NamedIndividual ,
                         ontouml:ClassStereotype ;
                rdfs:comment "A Quality is a particular type of intrinsic property that has a structured value. Qualities are things that existentially depend on the things they characterize, called their bearers."@en ;
                rdfs:seeAlso "https://ontouml.readthedocs.io/en/latest/classes/aspects/quality/index.html"^^xsd:anyURI .


###  https://w3id.org/ontouml#qualityNature
ontouml:qualityNature rdf:type owl:NamedIndividual ,
                               ontouml:OntologicalNature ;
                      rdfs:comment "Indicates that the restricted type includes quality individuals among its instances."@en .


###  https://w3id.org/ontouml#quantity
ontouml:quantity rdf:type owl:NamedIndividual ,
                          ontouml:ClassStereotype ;
                 rdfs:comment "Construct used to represent rigid concepts that provide an identity principle for their instances."@en ;
                 rdfs:seeAlso "https://ontouml.readthedocs.io/en/latest/classes/sortals/quantity/index.html"^^xsd:anyURI .


###  https://w3id.org/ontouml#quantityNature
ontouml:quantityNature rdf:type owl:NamedIndividual ,
                                ontouml:OntologicalNature ;
                       rdfs:comment "Indicates that the restricted type includes quantity individuals among its instances."@en .


###  https://w3id.org/ontouml#relator
ontouml:relator rdf:type owl:NamedIndividual ,
                         ontouml:ClassStereotype ;
                rdfs:comment "A construct used to represent truth-makers of material relations, i.e., the things that must exist for two or more individuals to be connected by material relations."@en ;
                rdfs:seeAlso "https://ontouml.readthedocs.io/en/latest/classes/sortals/relator/index.html"^^xsd:anyURI .


###  https://w3id.org/ontouml#relatorNature
ontouml:relatorNature rdf:type owl:NamedIndividual ,
                               ontouml:OntologicalNature ;
                      rdfs:comment "Indicates that the restricted type includes relator individuals among its instances."@en .


###  https://w3id.org/ontouml#role
ontouml:role rdf:type owl:NamedIndividual ,
                      ontouml:ClassStereotype ;
             rdfs:comment "A construct used to represent anti-rigid specializations of identity providers (Kind, Collective, Quantity, Relator, Mode, and Quantity) that are instantiated in relational contexts."@en ;
             rdfs:seeAlso "https://ontouml.readthedocs.io/en/latest/classes/sortals/role/index.html"^^xsd:anyURI .


###  https://w3id.org/ontouml#roleMixin
ontouml:roleMixin rdf:type owl:NamedIndividual ,
                           ontouml:ClassStereotype ;
                  rdfs:comment "The equivalent of Role for types that aggregate instances with different identity principles."@en ;
                  rdfs:seeAlso "https://ontouml.readthedocs.io/en/latest/classes/nonsortals/rolemixin/index.html"^^xsd:anyURI .


###  https://w3id.org/ontouml#shared
ontouml:shared rdf:type owl:NamedIndividual ,
                        ontouml:AggregationKind ;
               rdfs:comment "Indicates that the ontouml:Property has shared aggregation semantics."@en , 
               "The precise semantics of shared aggregation vary by application area and modeler."@en .


###  https://w3id.org/ontouml#situation
ontouml:situation rdf:type owl:NamedIndividual ,
                           ontouml:ClassStereotype ;
                  rdfs:comment "Can be used to represent certain configurations of entities that can be comprehended as a whole."@en .


###  https://w3id.org/ontouml#situationNature
ontouml:situationNature rdf:type owl:NamedIndividual ,
                                 ontouml:OntologicalNature ;
                        rdfs:comment "Indicates that the restricted type includes situation individuals among its instances."@en .


###  https://w3id.org/ontouml#subCollectionOf
ontouml:subCollectionOf rdf:type owl:NamedIndividual ,
                                 ontouml:RelationStereotype ;
                        rdfs:comment "A parthood relation between two collectives."@en ;
                        rdfs:seeAlso "https://ontouml.readthedocs.io/en/latest/relationships/aggregations/subCollectionOf/index.html"^^xsd:anyURI .


###  https://w3id.org/ontouml#subQuantityOf
ontouml:subQuantityOf rdf:type owl:NamedIndividual ,
                               ontouml:RelationStereotype ;
                      rdfs:comment "A parthood relation between two quantities."@en ;
                      rdfs:seeAlso "https://ontouml.readthedocs.io/en/latest/relationships/aggregations/subQuantityOf/index.html"^^xsd:anyURI .


###  https://w3id.org/ontouml#subkind
ontouml:subkind rdf:type owl:NamedIndividual ,
                         ontouml:ClassStereotype ;
                rdfs:comment "A Subkind is a construct used to represent rigid specializations of identity providers (Kind, Collective, Quantity, Relator, Mode, and Quantity). By default, its usage does not require a relational dependency."@en ;
                rdfs:seeAlso "https://ontouml.readthedocs.io/en/latest/classes/sortals/subkind/index.html"^^xsd:anyURI .


###  https://w3id.org/ontouml#termination
ontouml:termination rdf:type owl:NamedIndividual ,
                             ontouml:RelationStereotype .


###  https://w3id.org/ontouml#triggers
ontouml:triggers rdf:type owl:NamedIndividual ,
                          ontouml:RelationStereotype .


###  https://w3id.org/ontouml#type
ontouml:type rdf:type owl:NamedIndividual ,
                      ontouml:ClassStereotype ;
             rdfs:comment "The stereotype for high-order types in the OWL serialization."@en .


###  https://w3id.org/ontouml#typeNature
ontouml:typeNature rdf:type owl:NamedIndividual ,
                            ontouml:OntologicalNature ;
                   rdfs:comment "Indicates that the restricted type includes type individuals among its instances."@en .


#################################################################
#    Annotations
#################################################################

ontouml:containsModelElement rdfs:comment "Indicates the entities of type ontouml:ModelElement that composes an ontouml:Package."@en ,
                                          "Provides the elements contained by a given package in a given model. A model element is an elementary component of a model. It will be created when you create a shape in a diagram. An example of a model element is \"actor\"."@en ,
                                          "It is mapped to the OntoUML Metamodel's 'contents' relation between a Package and a ModelElement."@en .


ontouml:containsView rdfs:comment "Indicates the ontouml:ElementView entities that are part of a given ontouml:Diagram."@en .


ontouml:contents rdfs:comment "Identifies which entities of type ontouml:ElementView are part of a given ontouml:Diagram."@en ,
                              "The OntoUML Metamodel contains two contents relations, which are mapped to two different object properties in this vocabulary: containsModelElement and containsView. The contents object property aggregates both mentioned sub-properties in order to keep a clear relation to the metamodel even though it must not be directly used."@en .


#################################################################
#    General axioms
#################################################################

[ rdf:type owl:AllDisjointClasses ;
  owl:members ( ontouml:AggregationKind
                ontouml:Cardinality
                ontouml:OntologicalNature
                ontouml:OntoumlElement
                ontouml:Point
                ontouml:Stereotype
              )
] .


###  Generated by the OWL API (version 4.5.9.2019-02-01T07:24:44Z) https://github.com/owlcs/owlapi
